InhType.v
@@ -17,34 +17,34 @@ Definition ext {n} (f : 'I_n -> T) (k : nat) : T := oapp f inh (insub k).
 Lemma ext_add {x n} {f : 'I_n -> T} r : r != n ->
   ext (add f x) r = ext f r.
 Proof.
-  rewrite /ext. do ?insub_case; try slia. move=> ?? <- [/= ??? /double ? <- ?]. 
+  rewrite /ext. do ?case: insubP; try slia. move=> ?? <- [/= ??? /double ?<-?].
   rewrite add_lt //=; try slia. move=> ?/=. exact /congr1 /ord_inj.
 Qed.
 
 Lemma ext_add_n  {x n} {f : 'I_n -> T} :
   ext (add f x) n = x.
 Proof. 
-  rewrite /ext. insub_case; try slia. move=> [/=] ? L _ /esym E.
+  rewrite /ext. case: insubP; try slia. move=> [/=] ? L _ /esym E.
   case: _ / E L=> ?. by rewrite add_ord_max.
 Qed. 
 
 Lemma pred_ext {n} (f : 'I_n -> T) (p : pred T) (r : 'I_n) :
  p (ext f r) = p (f r).
 Proof.
-  case: r=> /= *. rewrite /ext. insub_case=> [*|]; try slia.
+  case: r=> /= *. rewrite /ext. case: insubP=> //= [*|]; try slia.
   exact /congr1 /congr1 /ord_inj.
 Qed.
 
 Lemma rel_ext {n x} (f : 'I_n -> T) (r : rel T) (a b : nat) :
-   ~ (rfield r inh) -> (r \o2 ext f) a b -> (r \o2 ext (add f x)) a b.
+   ~ (rfield r inh) -> (relpre (ext f) r) a b -> (relpre (ext (add f x)) r) a b.
 Proof.
-  rewrite /comp2=> H. case L: (a < n).
+  rewrite /relpre=> H /=. case L: (a < n).
   { rewrite ext_add //; try slia.
     case L': (b < n). 
     { rewrite ext_add //. slia. }
-    rewrite {2}/ext. do ?insub_case; try slia.
+    rewrite {2}/ext. do ?case: insubP; try slia.
     by move/1$/(codom_rfield _). }
-  rewrite {1}/ext. do ?insub_case; try slia.
+  rewrite {1}/ext. do ?case: insubP; try slia. 
   by move/1$/(dom_rfield _).
 Qed.
  
